theories/fin_maps.v
@@ -42,8 +42,10 @@ Class FinMap K M `{FMap M, ∀ A, Lookup K A (M A), ∀ A, Empty (M A), ∀ A,
   NoDup_map_to_list {A} (m : M A) : NoDup (map_to_list m);
   elem_of_map_to_list {A} (m : M A) i x :
     (i,x) ∈ map_to_list m ↔ m !! i = Some x;
-  lookup_omap {A B} (f : A → option B) m i : omap f m !! i = m !! i ≫= f;
-  lookup_merge {A B C} (f: option A → option B → option C) `{!DiagNone f} m1 m2 i :
+  lookup_omap {A B} (f : A → option B) (m : M A) i :
+    omap f m !! i = m !! i ≫= f; 
+  lookup_merge {A B C} (f : option A → option B → option C)
+      `{!DiagNone f} (m1 : M A) (m2 : M B) i :
     merge f m1 m2 !! i = f (m1 !! i) (m2 !! i)
 }.
 
@@ -943,7 +945,7 @@ Proof.
 Qed.
 
 Lemma elem_of_map_to_set_pair `{FinSet (K * A) C} (m : M A) i x :
-  (i,x) ∈ map_to_set pair m ↔ m !! i = Some x.
+  (i,x) ∈@{C} map_to_set pair m ↔ m !! i = Some x.
 Proof. rewrite elem_of_map_to_set. naive_solver. Qed.
 
 (** ** Induction principles *)
